proof/garble/equivAda.ec
@@ -7,135 +7,19 @@ require import Int.
 require import Bool.
 require import Array.
 
-require import Dkc.
+require import Hypothesis.
 require import GarbleTools.
 require import Garble.
-require AdvGarble.
-require AdvGarble_inter.
-
-
+require import Reduction.
+require import ReductionAda.
 
 lemma realEq :
-  forall (ADV <: Garble.Adv{AdvGarble.Adv, Dkc.Dkc, AdvGarble_inter.Inter}),
+  forall (ADV <: Garble.Adv{Red, DKC.Dkc}),
     equiv [
-      Dkc.Game(Dkc.Dkc, AdvGarble.Adv(ADV)).main ~
-      AdvGarble_inter.Game2(Dkc.Dkc, ADV).main
+      DKC.Game(DKC.Dkc, Red(ADV)).main ~
+      DKC.GameAda(DKC.Dkc, RedAda(ADV)).main
       : (glob ADV){1} = (glob ADV){2} ==> res{1} = res{2}
-    ]
+    ].
 proof.
-
-  intros ADV.
-  fun.
-  inline{1} Dkc.Game(Dkc.Dkc, AdvGarble.Adv(ADV)).preInit.
-  inline{2} AdvGarble_inter.Game2(Dkc.Dkc, ADV).preInit.
-  inline Dkc.Dkc.preInit.
-  inline{1} Dkc.Game(Dkc.Dkc, AdvGarble.Adv(ADV)).work.
-  inline{2} AdvGarble_inter.Game2(Dkc.Dkc, ADV).work.
-  inline AdvGarble.Adv(ADV).gen_queries.
-  inline AdvGarble.Adv(ADV).get_challenge.
-  inline AdvGarble.Adv(ADV).preInit.
-
-  inline {2} AdvGarble_inter.Game2(Dkc.Dkc, ADV).A.work.
-  inline {2} AdvGarble_inter.Inter(ADV, Dkc.Dkc).garble.
-  inline {2} AdvGarble_inter.Inter(ADV, Dkc.Dkc).query.
-  inline {2} AdvGarble_inter.Inter(ADV, Dkc.Dkc).garbD.
-  inline {2} AdvGarble_inter.Inter(ADV, Dkc.Dkc).garb.
-
-  inline {1} AdvGarble.Adv(ADV).garble_queries.
-  inline {1} AdvGarble.Adv(ADV).garble_answer.
-  inline {1} AdvGarble.Adv(ADV).query1.
-  inline {1} AdvGarble.Adv(ADV).query2.
-  inline {1} AdvGarble.Adv(ADV).garbD.
-  inline {1} AdvGarble.Adv(ADV).garb.
-
-  inline Dkc.Dkc.preInit.
-  inline Dkc.Dkc.get_challenge.
-  inline Dkc.Dkc.initialize.
-  inline Dkc.Dkc.encrypt.
-
-  wp. 
-
-  case (queryValid AdvGarble.Adv.query{1}).
-    rcondt{1} 21. admit.
-    rcondt{1} 36. admit.
-    rcondt{2} 21. admit.
-    wp.
-    call (answer{1}=answer{2} /\ (glob ADV){1} = (glob ADV){2}) (res{1}=res{2}).
-      fun true;smt.
-    wp.
-    while (
-      AdvGarble.Adv.l{1} = AdvGarble_inter.Inter.l{2} /\
-      AdvGarble.Adv.aa{1} = AdvGarble_inter.Inter.aa{2} /\
-      AdvGarble.Adv.bb{1} = AdvGarble_inter.Inter.bb{2} /\
-      AdvGarble.Adv.v{1} = AdvGarble_inter.Inter.v{2} /\
-      AdvGarble.Adv.xx{1} = AdvGarble_inter.Inter.xx{2} /\
-      AdvGarble.Adv.g{1} = AdvGarble_inter.Inter.g{2} /\
-      AdvGarble.Adv.t{1} = AdvGarble_inter.Inter.t{2} /\
-      AdvGarble.Adv.pp{1}=AdvGarble_inter.Inter.pp{2} /\
-      AdvGarble.Adv.a{1}=AdvGarble_inter.Inter.a{2} /\
-      AdvGarble.Adv.b{1}=AdvGarble_inter.Inter.b{2} /\
-      rand7{1} = rand3{2}
-    ).
-    wp.
-    app 6 6 : (
-      AdvGarble.Adv.l{1} = AdvGarble_inter.Inter.l{2} /\
-      AdvGarble.Adv.aa{1} = AdvGarble_inter.Inter.aa{2} /\
-      AdvGarble.Adv.bb{1} = AdvGarble_inter.Inter.bb{2} /\
-      AdvGarble.Adv.v{1} = AdvGarble_inter.Inter.v{2} /\
-      AdvGarble.Adv.xx{1} = AdvGarble_inter.Inter.xx{2} /\
-      AdvGarble.Adv.g{1} = AdvGarble_inter.Inter.g{2} /\
-      AdvGarble.Adv.t{1} = AdvGarble_inter.Inter.t{2} /\
-      AdvGarble.Adv.pp{1}=AdvGarble_inter.Inter.pp{2} /\
-      AdvGarble.Adv.a{1}=AdvGarble_inter.Inter.a{2} /\
-      AdvGarble.Adv.b{1}=AdvGarble_inter.Inter.b{2} /\
-      rand7{1} = rand3{2}
-    ). wp. skip. smt.
-    if.
-    smt.
-    wp.
-    app 3 3 : (
-      AdvGarble.Adv.l{1} = AdvGarble_inter.Inter.l{2} /\
-      AdvGarble.Adv.aa{1} = AdvGarble_inter.Inter.aa{2} /\
-      AdvGarble.Adv.bb{1} = AdvGarble_inter.Inter.bb{2} /\
-      AdvGarble.Adv.v{1} = AdvGarble_inter.Inter.v{2} /\
-      AdvGarble.Adv.xx{1} = AdvGarble_inter.Inter.xx{2} /\
-      AdvGarble.Adv.g{1} = AdvGarble_inter.Inter.g{2} /\
-      AdvGarble.Adv.t{1} = AdvGarble_inter.Inter.t{2} /\
-      AdvGarble.Adv.pp{1}=AdvGarble_inter.Inter.pp{2} /\
-      AdvGarble.Adv.a{1}=AdvGarble_inter.Inter.a{2} /\
-      AdvGarble.Adv.b{1}=AdvGarble_inter.Inter.b{2} /\
-      rand7{1} = rand3{2}
-    ). wp. skip. intros &1 &2 h. smt.
-    if. smt.
-
-    app 3 3 : (
-      AdvGarble.Adv.l{1} = AdvGarble_inter.Inter.l{2} /\
-      AdvGarble.Adv.aa{1} = AdvGarble_inter.Inter.aa{2} /\
-      AdvGarble.Adv.bb{1} = AdvGarble_inter.Inter.bb{2} /\
-      AdvGarble.Adv.v{1} = AdvGarble_inter.Inter.v{2} /\
-      AdvGarble.Adv.xx{1} = AdvGarble_inter.Inter.xx{2} /\
-      AdvGarble.Adv.g{1} = AdvGarble_inter.Inter.g{2} /\
-      AdvGarble.Adv.t{1} = AdvGarble_inter.Inter.t{2} /\
-      AdvGarble.Adv.pp{1}=AdvGarble_inter.Inter.pp{2} /\
-      AdvGarble.Adv.a{1}=AdvGarble_inter.Inter.a{2} /\
-      AdvGarble.Adv.b{1}=AdvGarble_inter.Inter.b{2} /\
-      rand7{1} = rand3{2}
-    ).
-
-
-
-
-  swap{1} 7 -6.
-
-  app 1 1 : (AdvGarble.Adv.query{1} = query{2}).
-  call ((glob ADV){1} = (glob ADV){2}) (res{1}=res{2} /\ (glob ADV){1} = (glob ADV){2}).
-    fun true;smt.
-  skip;smt.
-  
-  case (Garble.queryValid query{2}).
-
-  rcondt {1} 27;[admit|].
-  rcondt {1} 18;[admit|].
-  rcondt {2} 1;[intros &m;skip;smt|].
-  
+  admit.
 save.
