proof/garble/equivHybrid.ec
@@ -7,7 +7,21 @@ require import Int.
 require import Bool.
 require import Array.
 
-require import Dkc.
+require import Hypothesis.
 require import GarbleTools.
 require import Garble.
-require AdvGarble.
+require import RedAda.
+
+lemma realEq :
+  forall (ADV <: Garble.Adv{ReductionAda, DKC.Dkc, Garble.PrvInd}),
+    forall (l:int),
+    equiv [
+      DKC.GameAda(DKC.Dkc, RedAda(ADV)).work ~
+      DKC.GameAda(DKC.Dkc, RedAda(ADV)).work
+      : (glob ADV){1} = (glob ADV){2} /\
+      (!DKC.Dkc.b{1}) /\ (RedAda.l{1}=l) /\
+      (DKC.Dkc.b{2}) /\ (RedAda.l{2}=l+1) ==> res{1} = res{2}
+    ].
+proof.
+admit.
+save.
