proof/garble/theorem.ec
@@ -1,0 +1,27 @@
+require import Real.
+
+(*TODO Remove by Section*)
+require import Reduction.
+
+(*Hypothesis*)
+require import Hypothesis.
+
+(*Definition*)
+require import Garble.
+
+(*Lemmas*)
+require import CorrectionProof.
+require import ReductionProof.
+
+(*Theorem*)
+lemma GarbleCorrect :
+  forall (f : funct) , functCorrect f =>
+  forall (x : random) , randomCorrect f x =>
+  forall (i : input) , inputCorrect f i =>
+    let (g, ki, ko) = garble x f in
+    eval f i = decrypt ko (evalG g (encrypt ki i)) by [].
+
+lemma GarbleSecure :
+  exists (epsilon:real), epsilon > 0%r /\
+    forall (Adv<:Garble.Adv{DKC.Dkc,DKC.Game,Red}), forall &m,
+        `|Pr[Garble.Game(Garble.PrvInd(RandGarble), Adv).main()@ &m:res] - 1%r / 2%r| < epsilon by [].
