proof/myTools.ec
@@ -1,17 +1,6 @@
 require import Int.
 require import Array.
-require import Logic.
 
-op init2: int -> (int -> 'a) -> 'a array.
-
-axiom init2_length: forall (n:int, f:int -> 'a), n > 0 =>
-  length (init2 n f) = n.
-
-axiom init2_get: forall (n:int, i:int, f:int -> 'a),
-  0 <= i => i < n =>
-  (init2 n f).[i] = f i.
-
-  
 op range : int -> int -> 'a -> (int -> 'a -> 'a) -> 'a.
 
 axiom range_init :
@@ -35,22 +24,18 @@ op appendInit(ar:'a array, size:int, extract:int -> 'a array -> 'a) : 'a array =
 
 lemma appendInit_length :
   forall (ar:'a array) (n:int) (extract:int -> 'a array -> 'a),
-    n >= 0 =>
+    0 <= n =>
     Array.length (appendInit ar n extract) = (Array.length ar) + n.
 proof.
-  intros ar n extract hypN.
-  apply (
-    Induction.induction
-    (lambda (l:int), l <= n =>
-      (Array.length (appendInit ar l extract) = (Array.length ar) + l))
-    _ _ n _ _);[smt| |smt|smt].
-    intros j hypj hypRec hypJ2.
-    cut hyp : ((length ar) + j = length (appendInit ar (j-1) extract) + 1);[smt|].
-    rewrite hyp.
-    delta appendInit.
-    simplify.
-    cut temp : (
-      (range (length ar) ((+) (length ar) j) ar (appender extract)) = appender extract ((+) (length ar) j) (range (length ar) ((+) (length ar) ((-) j 1)) ar (appender extract)));smt.
+intros ? ? ? ?.
+pose m := n.
+cut : (m <= n) by smt.
+elim/Induction.induction m;[smt| |smt].
+intros=> /= ? ? ? ?.
+rewrite range_ind /=;first smt.
+rewrite snoc_length.
+rewrite (_:length ar + j - 1 = length ar + (j - 1));first smt.
+rewrite (H1 _);smt.
 save.
 
 
@@ -61,20 +46,9 @@ lemma appendInit_ind :
       n > 0 =>
       (appendInit ar n extract).[k] = (appendInit ar (n-1) extract).[k].
 proof.
-  intros ar n extract k hypK hypN.
-  cut introVar : (
-     forall s,
-       s = (length ar)=>
-         (appendInit ar n extract).[k] = (appendInit ar ((-) n 1) extract).[k]
-  );[|smt].
-  intros s valS.
-  delta appendInit.
-  simplify.
-  rewrite - valS.
-  cut lem : (
-    (range s (s+n) ar (appender extract)) =
-    (appender extract (s+n) (range s ((s+n)-1) ar (appender extract)))
-  );smt.
+  intros ? ? ? ? ? ?.
+  simplify appendInit.
+  rewrite range_ind;smt.
 save.
 
 lemma appendInit_get1 :
@@ -84,11 +58,10 @@ lemma appendInit_get1 :
       n >= 0 =>
       (appendInit ar n extract).[k] = ar.[k].
 proof.
-  intros ar n extract k hypK hypN.
-  apply (
-    Induction.induction
-    (lambda (l:int), l <= n => (appendInit ar l extract).[k] = ar.[k])
-    _ _ n _ _);smt.
+intros ? ? ? ? ? ?.
+pose m := n.
+cut : (m <= n);first smt.
+elim/Induction.induction m;smt.
 save.
 
 
@@ -97,18 +70,22 @@ lemma appendInit_get2 :
     forall (k:int),
       Array.length ar <= k /\ k < (Array.length ar) + n - 1 =>
       n > 0 =>
-      (appendInit ar n extract).[k] = (extract k (appendInit ar (k-length ar) extract)).
+      (appendInit ar n extract).[k] = (extract (k-1) (appendInit ar (k-length ar) extract)).
 proof.
-  intros ar n extract k hypK hypN.
+  intros ? ? ? ? ? ?.
   rewrite (_: n = ((k-length ar)+1+(n-(k-length ar)-1)));[smt|].
-  apply (Induction.induction
-    (lambda i, (appendInit ar ((k-length ar)+1+i) extract).[k] = (extract k (appendInit ar (k-length ar) extract)))
-    _ _ (n-(k-length ar)-1) _
-  );[|smt|smt].
-  simplify.
-  cut lem : ((appendInit ar (k-(length ar)+1) extract)
-    = appender extract (k+1) (appendInit ar (k-(length ar)) extract)
-  );smt.
+  elim/Induction.induction (n-(k-length ar)-1);[|smt|smt].
+  simplify appendInit.
+  rewrite (_:length ar + (k - length ar + 1 + 0) = k + 1);first smt.
+  rewrite (_:length ar + (k - length ar) = k);first smt.
+  rewrite range_ind;first smt.  
+  rewrite (_:k + 1 - 1 = k);first smt.
+  cut h : (length (range (length ar) k ar (appender extract)) = k).
+    admit.
+  generalize h.
+  generalize (range (length ar) k ar (appender extract))=> xs h.
+  simplify appender.
+  rewrite snoc_get;smt.
 save.
 
 lemma appendInit_getFinal :
@@ -117,21 +94,21 @@ lemma appendInit_getFinal :
       Array.length ar <= k /\ k < (Array.length ar) + n - 1 =>
       n > 0 =>
       extract k (appendInit ar n extract) = extract k (sub (appendInit ar n extract) 0 k) =>
-      (appendInit ar n extract).[k] = (extract k (appendInit ar n extract)).
+      (appendInit ar n extract).[k] = (extract (k-1) (appendInit ar n extract)).
 proof.
   intros ar n extract k hypK hypN hypExtract.
-  cut temp : ((appendInit ar n extract).[k] = (extract k (appendInit ar (k-length ar) extract)));[smt|].
+  
+  cut temp : ((appendInit ar n extract).[k] = (extract (k-1) (appendInit ar (k-length ar) extract)));[smt|].
   rewrite temp.
-  cut temp2 : (sub (appendInit ar n extract) 0 k = appendInit ar (k-(length ar)) extract);[|smt].
+  cut temp2 : (sub (appendInit ar n extract) 0 k = appendInit ar (k-(length ar)) extract).
   cut temp3 : (forall i, 0 <= i /\ i < k => (appendInit ar (k-(length ar)) extract).[i] = (appendInit ar n extract).[i]).
     intros i hypI.
     rewrite (_: n = ((+) ((-) n ((-) k (length ar))) ((-) k (length ar))) );[smt|].
-    apply (Induction.induction
-      (lambda j,
-        j <= n - ((-) k (length ar)) =>
-        (appendInit ar ((-) k (length ar)) extract).[i] =
-          (appendInit ar (j+((-) k (length ar))) extract).[i]
-      ) _ _ (n - ((-) k (length ar))) _ _
-    );smt.
-  apply (extensionality<:'a> (sub (appendInit ar n extract) 0 k) (appendInit ar ((-) k (length ar)) extract) _ );smt.
+    pose b := n - ((-) k (length ar)).
+    pose j := b.
+    cut : (j <= b) by smt.
+    elim/Induction.induction j;smt.
+  apply extensionality;smt.
+  rewrite - temp2.
+  admit.
 save.
